Wavelet/Simulation.lean
@@ -1,0 +1,227 @@
+import Mathlib.Data.List.Basic
+import Mathlib.Logic.Relation
+
+import Wavelet.Op
+import Wavelet.Seq
+import Wavelet.Dataflow
+import Wavelet.Compile
+import Wavelet.Lemmas
+
+open Wavelet.Op
+
+universe u
+variable (Op : Type u) (χ : Type u) (V S)
+variable [instArity : Arity Op] [DecidableEq χ] [instInterp : Interp Op V S]
+
+namespace Wavelet.Simulation
+
+open Op Seq Dataflow Compile
+
+/-- Defines refinement of two transition systems in general. -/
+def Refines
+  {T : Type v} {S : Type w}
+  (c₁ : T) (c₂ : S)
+  (R : T → S → Prop)
+  (Step₁ : T → T → Prop)
+  (Step₂ : S → S → Prop) :=
+  R c₁ c₂ ∧
+  (∀ c₁ c₂ c₁',
+    R c₁ c₂ →
+    Step₁ c₁ c₁' →
+    ∃ c₂', Step₂ c₂ c₂' ∧ R c₁' c₂')
+
+/-- Specific case for a Seq config to refine a dataflow config. -/
+def SeqRefinesDataflow
+  [DecidableEq χ₁] [DecidableEq χ₂]
+  (c₁ : Seq.Config Op χ₁ V S m n)
+  (c₂ : Dataflow.Config Op χ₂ V S m n)
+  (R : Seq.Config Op χ₁ V S m n → Dataflow.Config Op χ₂ V S m n → Prop) : Prop :=
+  Refines c₁ c₂ R (Config.Step Op χ₁ V S) (Config.StepPlus Op χ₂ V S)
+
+def SimR
+  (hnz : m > 0 ∧ n > 0)
+  (ec : Seq.Config Op χ V S m n)
+  (pc : Dataflow.Config Op (ChanName χ) V S m n) : Prop :=
+  ec.state = pc.state ∧
+  ∃ (rest : AtomicProcs Op (ChanName χ) V)
+    (carryInLoop : Bool)
+    (ctxLeft ctxCurrent ctxRight : AtomicProcs Op (ChanName χ) V),
+    -- Some invariants about the form of the processes
+    pc.proc.atoms = compileFn.initCarry _ _ _ ec.fn carryInLoop :: rest ∧
+    (compileFn Op χ V S hnz ec.fn).atoms = compileFn.initCarry _ _ _ ec.fn false :: rest ∧
+    rest = ctxLeft ++ ctxCurrent ++ ctxRight ∧
+    -- TODO: include this
+    -- (∀ vals, ec.expr = .ret vals → ¬ carryInLoop ∧ ctxCurrent = [] ∧ ctxRight = []) ∧
+    (∀ expr, ec.expr = .cont expr → carryInLoop ∧
+      expr.WellFormed _ _ ec.definedVars ∧
+      compileExpr Op χ V S hnz ec.definedVars ec.pathConds expr = ctxCurrent) ∧
+    (∀ var val, ec.vars.getVar _ _ var = some val →
+      pc.chans.IsSingleton _ _ (.var var ec.pathConds) val) ∧
+    (∀ cond ∈ ec.pathConds, pc.chans.IsSingleton _ _ (.merge_cond cond.2) instInterp.trueVal) ∧
+    (∀ i, (h : i < ec.pathConds.length) →
+      compileExpr.brMerge _ _ _ m n (ec.pathConds[i]'h).2 (ec.pathConds.drop i) ∈ pc.proc.atoms) ∧
+    (∀ var ∈ ec.definedVars, ∃ val, ec.vars.getVar _ _ var = some val) ∧
+    (∀ name : ChanName χ, match name with
+      | .var _ pathConds => pathConds ≠ ec.pathConds → pc.chans.IsEmpty _ _ name
+      | .merge_cond v => (∀ cond ∈ ec.pathConds, v ≠ cond.2) → pc.chans.IsEmpty _ _ name
+      | _ => pc.chans.IsEmpty _ _ name)
+
+theorem pop_singleton {chans : ChanMap χ V}
+  (hsingleton : chans.IsSingleton _ _ name val) :
+  ∃ chans',
+    chans.popVal _ _ name = some (val, chans') ∧
+    chans'.getBuf _ _ name = [] ∧
+    ∀ name', name' ≠ name → chans'.getBuf _ _ name' = chans.getBuf _ _ name'
+:= sorry
+
+theorem pop_singletons
+  {chans : ChanMap χ V}
+  {names : Vector χ n}
+  (prop : χ → V → Prop)
+  (hsingletons : ∀ name ∈ names, ∃ val, chans.IsSingleton _ _ name val ∧ prop name val)
+  (hdisj : names.toList.Nodup) :
+  ∃ vals chans',
+    chans.popVals _ _ names = some (vals, chans') ∧
+    List.Forall₂ prop names.toList vals.toList ∧
+    (∀ name ∈ names, chans'.IsEmpty _ _ name) ∧
+    (∀ name, name ∉ names → chans'.getBuf _ _ name = chans.getBuf _ _ name)
+:= sorry
+
+theorem sim_step_br
+  {cond}
+  (hnz : m > 0 ∧ n > 0)
+  (ec ec' : Seq.Config Op χ V S m n)
+  (pc : Dataflow.Config Op (ChanName χ) V S m n)
+  (hsim : SimR _ _ _ _ hnz ec pc)
+  (hstep : Config.Step Op χ V S ec ec')
+  (hbr : ec.expr = .cont (.br cond left right)) :
+  ∃ pc',
+    Config.StepPlus Op (ChanName χ) V S pc pc' ∧
+    SimR _ _ _ _ hnz ec' pc' := by
+  have ⟨
+    heq_state,
+    ⟨
+      rest, carryInLoop, ctxLeft, ctxCurrent, ctxRight,
+      hatoms,
+      hcomp_fn,
+      hrest,
+      hcont,
+      hlive_vars,
+      hpath_conds,
+      hmerges,
+      hdefined_vars,
+      hempty_names,
+    ⟩,
+  ⟩ := hsim
+  have ⟨hcarryInLoop, hwf_expr, hcurrent⟩ := hcont (.br cond left right) hbr
+  simp [compileExpr] at hcurrent
+
+  -- Deduce some facts from `hstep`
+  cases hstep with
+  | step_ret hexpr => simp [hbr] at hexpr
+  | step_tail hexpr => simp [hbr] at hexpr
+  | step_op hexpr => simp [hbr] at hexpr
+  | step_br hexpr hcond =>
+    rename_i condVal _ _ cond'
+    simp [hbr] at hexpr
+    have heq_cond' := hexpr.1
+    subst heq_cond'
+
+    -- Pop `cond` and run the first `fork`
+    have hcondVal : pc.chans.IsSingleton _ _ (.var cond ec.pathConds) condVal
+      := hlive_vars cond condVal hcond
+    have ⟨chans', hpop_condVal, hchans'⟩ := pop_singleton _ _ hcondVal
+    have hmem_fork :
+      .fork (compileExpr.varName χ ec.pathConds cond)
+        #v[
+          .switch_cond (compileExpr.varName χ ec.pathConds cond),
+          .merge_cond (compileExpr.varName χ ec.pathConds cond),
+        ]
+      ∈ pc.proc.atoms
+    := by grind
+    generalize hpc₁ :
+      { pc with
+        chans :=
+          .pushVals _ _
+            #v[
+              .switch_cond (compileExpr.varName χ ec.pathConds cond),
+              (compileExpr.varName χ ec.pathConds cond).merge_cond,
+            ]
+            (Vector.replicate 2 condVal)
+            chans',
+        : Dataflow.Config _ _ _ _ _ _ } = pc₁
+    have hstep₁ :
+      Dataflow.Config.Step _ _ _ _ pc pc₁
+    := by
+      apply step_eq
+      apply Dataflow.Config.Step.step_fork hmem_fork hpop_condVal
+      simp [← hpc₁]
+
+    -- Run the switch
+    have hmem_switch :
+      .switch
+        (.switch_cond (compileExpr.varName χ ec.pathConds cond))
+        (compileExpr.allVars χ ec.definedVars ec.pathConds)
+        (compileExpr.allVars χ ec.definedVars
+          ((true, compileExpr.varName χ ec.pathConds cond) :: ec.pathConds))
+        (compileExpr.allVars χ ec.definedVars
+          ((false, compileExpr.varName χ ec.pathConds cond) :: ec.pathConds))
+      ∈ pc₁.proc.atoms
+    := by grind
+    have hcondVal₁ :
+      pc₁.chans.IsSingleton _ _ (.switch_cond (compileExpr.varName χ ec.pathConds cond)) condVal
+    := sorry
+    have ⟨chans'', hpop_condVal₁, hchans''⟩ := pop_singleton _ _ hcondVal₁
+
+    have hallVars_lookup :
+      ∀ name ∈ compileExpr.allVars χ ec.definedVars ec.pathConds,
+        ∃ val, chans''.IsSingleton _ _ name val ∧
+          (∃ var, name = .var var ec.pathConds ∧ ec.vars var = some val)
+    := sorry
+    have hallVars_disj :
+      (compileExpr.allVars χ ec.definedVars ec.pathConds).toList.Nodup
+    := sorry -- from well-formedness
+
+    have ⟨inputVals, chans''', hpop_inputVals, _⟩ := pop_singletons _ _ _ hallVars_lookup hallVars_disj
+
+    generalize hpc₂ :
+      { pc with
+        chans :=
+          if Interp.asBool Op S condVal = true then
+            ChanMap.pushVals (ChanName χ) V
+              (compileExpr.allVars χ ec.definedVars ((true, compileExpr.varName χ ec.pathConds cond) :: ec.pathConds))
+              inputVals chans'''
+          else
+            ChanMap.pushVals (ChanName χ) V
+              (compileExpr.allVars χ ec.definedVars ((false, compileExpr.varName χ ec.pathConds cond) :: ec.pathConds))
+              inputVals chans'''
+      } = pc₂
+    have hstep₂ :
+      Dataflow.Config.Step _ _ _ _ pc₁ pc₂
+    := by
+      apply step_eq
+      apply Dataflow.Config.Step.step_switch hmem_switch hpop_condVal₁ hpop_inputVals
+      simp [← hpc₁, ← hpc₂]
+
+    -- have pc₁.IsSingleton _ _ (.var cond ec.pathConds) condVal
+    -- := by
+    --   simp [hpc₁]
+    --   exact hchans' _ rfl
+
+    -- have hmem_steer₂ :
+    --   AtomicProc.steer false
+    --     (compileExpr.varName χ ec.pathConds cond)
+    --     (compileExpr.allVars χ ec.definedVars ec.pathConds)
+    --     (compileExpr.allVars χ ec.definedVars ((false, compileExpr.varName χ ec.pathConds cond) :: ec.pathConds))
+    --   ∈ pc.proc.atoms
+    -- := by grind
+
+    -- have :
+    --   Dataflow.Config.Step _ _ _ _ pc
+    --     { pc with
+
+    --     }
+    -- := sorry
+    sorry
+
+end Wavelet.Simulation
